more

Weidenbach_Book/IsaSAT_CDCL.thy
@@ -79,10 +79,6 @@ sepref_thm cdcl_twl_o_prog_wl_D_fast_code
   unfolding cdcl_twl_o_prog_wl_D_heur_def PR_CONST_def
   unfolding get_conflict_wl_is_None get_conflict_wl_is_None_heur_alt_def[symmetric]
   supply [[goals_limit = 1]] isasat_fast_def[simp]
-       apply sepref_dbg_keep
-  apply sepref_dbg_trans_keep
-  apply sepref_dbg_trans_step_keep
-  apply sepref_dbg_side_unfold
   by sepref
 
 concrete_definition (in -) cdcl_twl_o_prog_wl_D_fast_code
@@ -99,47 +95,6 @@ lemma (in isasat_input_ops) twl_st_heur_count_decided_st_alt_def:
   shows \<open>(S, T) \<in> twl_st_heur \<Longrightarrow> count_decided_st S = count_decided (get_trail_wl T)\<close>
   unfolding count_decided_st_def twl_st_heur_def
   by (cases S) auto
-
-lemma cdcl_twl_o_prog_wl_D_heur_cdcl_twl_o_prog_wl_D:
-  \<open>(cdcl_twl_o_prog_wl_D_heur, cdcl_twl_o_prog_wl_D) \<in> twl_st_heur \<rightarrow>\<^sub>f
-     \<langle>bool_rel \<times>\<^sub>f twl_st_heur\<rangle>nres_rel\<close>
-  unfolding cdcl_twl_o_prog_wl_D_heur_def cdcl_twl_o_prog_wl_D_def
-    get_conflict_wl_is_None
-  apply (intro frefI nres_relI)
-  apply (refine_vcg
-      decide_wl_or_skip_D_heur_decide_wl_or_skip_D[THEN fref_to_Down]
-      skip_and_resolve_loop_wl_D_heur_skip_and_resolve_loop_wl_D[THEN fref_to_Down]
-      backtrack_wl_D_nlit_backtrack_wl_D[THEN fref_to_Down])
-  subgoal
-   by (auto simp: twl_st_heur_state_simp
-     get_conflict_wl_is_None_heur_get_conflict_wl_is_None[THEN fref_to_Down_unRET_Id])
-  subgoal by (auto simp: twl_st_heur_state_simp twl_st_heur_count_decided_st_alt_def)
-  subgoal by (auto simp: twl_st_heur_state_simp twl_st_heur_twl_st_heur_conflict_ana)
-  subgoal by (auto simp: twl_st_heur_state_simp)
-  subgoal by (auto simp: twl_st_heur_state_simp)
-  done
-
-
-paragraph \<open>Combining Together: Full Strategy\<close>
-
-definition (in isasat_input_ops) cdcl_twl_stgy_prog_wl_D_heur
-   :: \<open>twl_st_wl_heur \<Rightarrow> twl_st_wl_heur nres\<close>
-where
-  \<open>cdcl_twl_stgy_prog_wl_D_heur S\<^sub>0 =
-  do {
-    do {
-      (brk, T) \<leftarrow> WHILE\<^sub>T
-        (\<lambda>(brk, _). \<not>brk)
-        (\<lambda>(brk, S).
-        do {
-          T \<leftarrow> unit_propagation_outer_loop_wl_D_heur S;
-          cdcl_twl_o_prog_wl_D_heur T
-        })
-        (False, S\<^sub>0);
-      RETURN T
-    }
-  }
-  \<close>
 
 lemma twl_st_heur''D_twl_st_heurD:
   assumes H: \<open>(\<And>\<D> r. f \<in> twl_st_heur'' \<D> r \<rightarrow>\<^sub>f \<langle>twl_st_heur'' \<D> r\<rangle> nres_rel)\<close>
@@ -165,6 +120,110 @@ proof -
       done
     done
 qed
+
+
+lemma twl_st_heur'''D_twl_st_heurD:
+  assumes H: \<open>(\<And>r. f \<in> twl_st_heur''' r \<rightarrow>\<^sub>f \<langle>twl_st_heur''' r\<rangle> nres_rel)\<close>
+  shows \<open>f \<in> twl_st_heur \<rightarrow>\<^sub>f \<langle>twl_st_heur\<rangle> nres_rel\<close>  (is \<open>_ \<in> ?A B\<close>)
+proof -
+  obtain f1 f2 where f: \<open>f = (f1, f2)\<close>
+    by (cases f) auto
+  show ?thesis
+    unfolding f
+    apply (simp only: fref_def twl_st_heur'_def nres_rel_def in_pair_collect_simp)
+    apply (intro conjI impI allI)
+    subgoal for x y
+      using assms[of \<open>length (get_clauses_wl_heur x)\<close>,
+        unfolded ref_def twl_st_heur'_def nres_rel_def in_pair_collect_simp f,
+        rule_format] unfolding f
+      apply (simp only: fref_def twl_st_heur'_def nres_rel_def in_pair_collect_simp)
+      apply (drule spec[of _ x])
+      apply (drule spec[of _ y])
+      apply simp
+      apply (rule "weaken_\<Down>'"[of _ \<open>twl_st_heur''' (length (get_clauses_wl_heur x))\<close>])
+      apply (fastforce simp: twl_st_heur'_def)+
+      done
+    done
+qed
+
+
+lemma twl_st_heur'''D_twl_st_heurD_prod:
+  assumes H: \<open>(\<And>r. f \<in> twl_st_heur''' r \<rightarrow>\<^sub>f \<langle>A \<times>\<^sub>r twl_st_heur''' r\<rangle> nres_rel)\<close>
+  shows \<open>f \<in> twl_st_heur \<rightarrow>\<^sub>f \<langle>A \<times>\<^sub>r twl_st_heur\<rangle> nres_rel\<close>  (is \<open>_ \<in> ?A B\<close>)
+proof -
+  obtain f1 f2 where f: \<open>f = (f1, f2)\<close>
+    by (cases f) auto
+  show ?thesis
+    unfolding f
+    apply (simp only: fref_def twl_st_heur'_def nres_rel_def in_pair_collect_simp)
+    apply (intro conjI impI allI)
+    subgoal for x y
+      using assms[of \<open>length (get_clauses_wl_heur x)\<close>,
+        unfolded ref_def twl_st_heur'_def nres_rel_def in_pair_collect_simp f,
+        rule_format] unfolding f
+      apply (simp only: fref_def twl_st_heur'_def nres_rel_def in_pair_collect_simp)
+      apply (drule spec[of _ x])
+      apply (drule spec[of _ y])
+      apply simp
+      apply (rule "weaken_\<Down>'"[of _ \<open>A \<times>\<^sub>r twl_st_heur''' (length (get_clauses_wl_heur x))\<close>])
+      apply (fastforce simp: twl_st_heur'_def)+
+      done
+    done
+qed
+
+lemma cdcl_twl_o_prog_wl_D_heur_cdcl_twl_o_prog_wl_D:
+  \<open>(cdcl_twl_o_prog_wl_D_heur, cdcl_twl_o_prog_wl_D) \<in> twl_st_heur \<rightarrow>\<^sub>f
+     \<langle>bool_rel \<times>\<^sub>f twl_st_heur\<rangle>nres_rel\<close>
+proof -
+  have [refine0]: \<open>(x, y) \<in> twl_st_heur \<Longrightarrow>
+           (x, y)
+           \<in> {(S, T).
+               (S, T) \<in> twl_st_heur_conflict_ana \<and>
+               length (get_clauses_wl_heur S) =
+               length (get_clauses_wl_heur x)}\<close> for x y
+    by (auto simp: twl_st_heur_state_simp twl_st_heur_twl_st_heur_conflict_ana)
+  show ?thesis
+    unfolding cdcl_twl_o_prog_wl_D_heur_def cdcl_twl_o_prog_wl_D_def
+      get_conflict_wl_is_None
+    apply (intro frefI nres_relI)
+    apply (refine_vcg
+        decide_wl_or_skip_D_heur_decide_wl_or_skip_D[THEN twl_st_heur'''D_twl_st_heurD_prod,
+             THEN fref_to_Down]
+        skip_and_resolve_loop_wl_D_heur_skip_and_resolve_loop_wl_D[THEN fref_to_Down]
+        backtrack_wl_D_nlit_backtrack_wl_D[THEN fref_to_Down])
+    subgoal
+      by (auto simp: twl_st_heur_state_simp
+          get_conflict_wl_is_None_heur_get_conflict_wl_is_None[THEN fref_to_Down_unRET_Id])
+    subgoal by (auto simp: twl_st_heur_state_simp twl_st_heur_count_decided_st_alt_def)
+    subgoal by (auto simp: twl_st_heur_state_simp twl_st_heur_twl_st_heur_conflict_ana)
+    subgoal by (auto simp: twl_st_heur_state_simp)
+    subgoal by (auto simp: twl_st_heur_state_simp)
+    subgoal by (auto simp: twl_st_heur_state_simp)
+    done
+qed
+
+
+paragraph \<open>Combining Together: Full Strategy\<close>
+
+definition (in isasat_input_ops) cdcl_twl_stgy_prog_wl_D_heur
+   :: \<open>twl_st_wl_heur \<Rightarrow> twl_st_wl_heur nres\<close>
+where
+  \<open>cdcl_twl_stgy_prog_wl_D_heur S\<^sub>0 =
+  do {
+    do {
+      (brk, T) \<leftarrow> WHILE\<^sub>T
+        (\<lambda>(brk, _). \<not>brk)
+        (\<lambda>(brk, S).
+        do {
+          T \<leftarrow> unit_propagation_outer_loop_wl_D_heur S;
+          cdcl_twl_o_prog_wl_D_heur T
+        })
+        (False, S\<^sub>0);
+      RETURN T
+    }
+  }
+  \<close>
+
 
 theorem unit_propagation_outer_loop_wl_D_heur_unit_propagation_outer_loop_wl_D:
   \<open>(unit_propagation_outer_loop_wl_D_heur, unit_propagation_outer_loop_wl_D) \<in>
@@ -204,215 +263,11 @@ prepare_code_thms (in -) cdcl_twl_stgy_prog_wl_D_code_def
 
 lemmas cdcl_twl_stgy_prog_wl_D_code[sepref_fr_rules] =
    cdcl_twl_stgy_prog_wl_D_code.refine[of \<A>\<^sub>i\<^sub>n]
-end
-(*
-definition (in -)isasat_fast2 where
-  \<open>isasat_fast2 = isasat_fast\<close>
-
-
-definition (in -) isasat_fast_clss :: \<open>_ \<Rightarrow> bool\<close> where
-  \<open>isasat_fast_clss = (\<lambda>(_, N). length N \<le> uint32_max)\<close>
-
-definition (in -) isasat_fast_clss_dom :: \<open>_ \<Rightarrow> bool\<close> where
-  \<open>isasat_fast_clss_dom = (\<lambda>N. \<forall>i\<in>#dom_m N. i < uint32_max)\<close>
-
-
-lemma (in -) isasat_fast_clss_dom:
-  \<open>(RETURN o isasat_fast_clss, RETURN o isasat_fast_clss_dom) \<in>
-      \<langle>Id\<rangle>clauses_l_fmat \<rightarrow>\<^sub>f \<langle>bool_rel\<rangle>nres_rel\<close>
-  apply (intro frefI nres_relI)
-  apply (auto simp:  clauses_ll_assn_def list_fmap_rel_def isasat_fast_clss_dom_def
-      isasat_fast_clss_def)
-  apply (subst (asm)(4) eq_commute)
-  apply auto
-  apply (case_tac \<open>dom_m y\<close>)
-   apply (auto simp: uint_max_def)
-  apply (subst (asm)(4) eq_commute)
-  apply auto
-  done
-
-definition (in -) isasat_fast_code :: \<open>twl_st_wll_trail_fast \<Rightarrow> bool\<close> where
-  \<open>isasat_fast_code = (\<lambda>(M', (N', _, n), _). n < uint32_max)\<close>
-
-
-lemma (in -)isasat_fast_clss_hnr[sepref_fr_rules]:
-  \<open>(return o (\<lambda>(N, _, n). n \<le> uint32_max), RETURN o isasat_fast_clss) \<in>
-       isasat_clauses_assn\<^sup>k \<rightarrow>\<^sub>a bool_assn\<close>
-  by sepref_to_hoare
-    (sep_auto simp: isasat_fast_clss_def min_def
-      isasat_fast2_def isasat_fast_code_def clauses_ll_assn_def
-      hr_comp_def list_fmap_rel_def arlO_assn_def arl_assn_def
-      is_array_list_def list_rel_imp_same_length[symmetric]
-      dest: heap_list_add_same_length
-      elim!: mod_starE
-      split: if_splits)
-
-lemma isasat_fast_clss_dom_hnr [sepref_fr_rules]:
-\<open>((return \<circ>\<circ> case_prod) (\<lambda>N (_, n). n \<le> uint_max),
-     RETURN \<circ> isasat_fast_clss_dom)
-    \<in> (clauses_ll_assn)\<^sup>k \<rightarrow>\<^sub>a bool_assn\<close>
-  using isasat_fast_clss_hnr[FCOMP isasat_fast_clss_dom] unfolding clauses_ll_assn_def[symmetric]
-  .
-
-lemma (in -)isasat_fast2_alt_def:
-  \<open>isasat_fast2 = (\<lambda>(M,N,_). isasat_fast_clss_dom N)\<close>
-  by (auto simp: isasat_fast2_def isasat_fast_clss_dom_def) *)
-
-
-context isasat_input_bounded_nempty
-begin
-
-(* declare isasat_fast_slow_code.refine[sepref_fr_rules] *)
-
-(* sepref_register isasat_fast2
-sepref_thm isasat_fast2_code
-  is \<open>RETURN o isasat_fast2\<close>
-  :: \<open>isasat_bounded_assn\<^sup>k \<rightarrow>\<^sub>a bool_assn\<close>
-  supply [[goals_limit=1]]
-  unfolding isasat_fast2_alt_def isasat_bounded_assn_def
-  by sepref
-
-concrete_definition (in -) isasat_fast2_code
-  uses isasat_input_bounded_nempty.isasat_fast2_code.refine_raw
-  is \<open>(?f, _) \<in> _\<close>
-
-prepare_code_thms (in -) isasat_fast2_code_def
-
-lemmas isasat_fast2_code[sepref_fr_rules] =
-   isasat_fast2_code.refine[OF isasat_input_bounded_nempty_axioms] *)
 
 sepref_register cdcl_twl_stgy_prog_wl_D_heur
 
-(* definition (in isasat_input_ops) cdcl_twl_stgy_prog_break_wl_D_heur_break
-   :: \<open>twl_st_wl_heur \<Rightarrow> twl_st_wl_heur nres\<close>
-where
-  \<open>cdcl_twl_stgy_prog_break_wl_D_heur_break S\<^sub>0 =
-  do {
-    let b = isasat_fast2 S\<^sub>0;
-    (b, brk, T) \<leftarrow> WHILE\<^sub>T\<^bsup>\<lambda>(b, brk, S). (b \<longrightarrow> \<not>brk \<longrightarrow>isasat_fast2 S)\<^esup>
-        (\<lambda>(b, brk, _). b \<and> \<not>brk)
-        (\<lambda>(b, brk, S).
-        do {
-          ASSERT (b \<and> \<not>brk);
-          T \<leftarrow> unit_propagation_outer_loop_wl_D_heur S;
-          ASSERT(isasat_fast2 T);
-          (brk, T) \<leftarrow> cdcl_twl_o_prog_wl_D_heur T;
-          b \<leftarrow> RETURN (isasat_fast2 T);
-          RETURN (b, brk, T)
-        })
-        (b, False, S\<^sub>0);
-    if brk then isasat_fast_slow T
-    else do {
-        T' \<leftarrow> isasat_fast_slow T;
-        cdcl_twl_stgy_prog_wl_D_heur T'
-    }
-  }\<close> *)
-(*
-sepref_register isasat_fast_slow
-sepref_thm cdcl_twl_stgy_prog_wl_D_fast_code
-  is \<open>PR_CONST cdcl_twl_stgy_prog_break_wl_D_heur_break\<close>
-  :: \<open>[isasat_fast]\<^sub>a isasat_bounded_assn\<^sup>d \<rightarrow> isasat_unbounded_assn\<close>
-  unfolding cdcl_twl_stgy_prog_break_wl_D_heur_break_def PR_CONST_def
-  supply [[goals_limit = 1]] isasat_input_bounded_nempty_axioms[intro] isasat_fast2_def[simp]
-  by sepref
-
-concrete_definition (in -) cdcl_twl_stgy_prog_wl_D_fast_code
-   uses isasat_input_bounded_nempty.cdcl_twl_stgy_prog_wl_D_fast_code.refine_raw
-   is \<open>(?f,_)\<in>_\<close>
-
-prepare_code_thms (in -) cdcl_twl_stgy_prog_wl_D_fast_code_def
-
-lemmas cdcl_twl_stgy_prog_wl_D_fast_code[sepref_fr_rules] =
-   cdcl_twl_stgy_prog_wl_D_fast_code.refine[of \<A>\<^sub>i\<^sub>n] *)
-
-(* definition  (in -)isasat_fast_wl where
-  \<open>isasat_fast_wl S = (\<forall>L\<in>#dom_m (get_clauses_wl S). L < uint_max)\<close>
-
-lemma twl_st_heur_isasat_fast_wl:
-   \<open>(x, y) \<in> twl_st_heur \<Longrightarrow> isasat_fast_wl y = isasat_fast2 x\<close>
-  by (auto simp: isasat_fast2_def twl_st_heur_state_simp twl_st_heur_def isasat_fast_wl_def)
-term isasat_fast_slow
-
-lemma cdcl_twl_stgy_prog_break_wl_D_alt_def:
-  \<open>cdcl_twl_stgy_prog_break_wl_D S\<^sub>0 =
-  do {
-    b \<leftarrow> SPEC (\<lambda>_. True);
-    (b, brk, T) \<leftarrow> WHILE\<^sub>T\<^bsup>\<lambda>(b, brk, T). cdcl_twl_stgy_prog_wl_inv S\<^sub>0 (brk, T) \<and>
-          literals_are_\<L>\<^sub>i\<^sub>n T\<^esup>
-        (\<lambda>(b, brk, _). b \<and> \<not>brk)
-        (\<lambda>(b, brk, S).
-        do {
-          ASSERT(b);
-          T \<leftarrow> unit_propagation_outer_loop_wl_D S;
-          (brk, T) \<leftarrow> cdcl_twl_o_prog_wl_D T;
-          b \<leftarrow>  SPEC (\<lambda>_. True);
-          RETURN(b, brk, T)
-        })
-        (b, False, S\<^sub>0);
-    if brk then RETURN (isasat_fast_slow_wl_D T)
-    else do {
-        let T' = isasat_fast_slow_wl_D T;
-        cdcl_twl_stgy_prog_wl_D T'
-     }
-  }\<close>
-  unfolding Let_def cdcl_twl_stgy_prog_break_wl_D_def isasat_fast_slow_wl_D_def id_apply
-  by (auto simp: Let_def)
-
-lemma cdcl_twl_stgy_prog_wl_D_heur_break_cdcl_twl_stgy_prog_wl_D:
-  \<open>(cdcl_twl_stgy_prog_break_wl_D_heur_break,
-     cdcl_twl_stgy_prog_break_wl_D) \<in>
-         twl_st_heur \<rightarrow>\<^sub>f \<langle>twl_st_heur\<rangle>nres_rel\<close>
-proof -
-  have H1: \<open>
-    (isasat_fast2 x, b) \<in> bool_rel \<Longrightarrow>
-    (x, y) \<in> twl_st_heur \<Longrightarrow>
-    ((isasat_fast2 x, False, x), b, False, y) \<in> {(b, b'). b = b' \<and>
-       (b \<longrightarrow> isasat_fast2 x)} \<times>\<^sub>r bool_rel \<times>\<^sub>r twl_st_heur\<close> for b x y
-    by auto
-  have H2:
-    \<open>(x, y) \<in> twl_st_heur \<Longrightarrow>
-    (isasat_fast2 x, isasat_fast_wl y) \<in> {(b, b'). b = b' \<and>
-       (b \<longrightarrow> isasat_fast2 x)}\<close> for x y
-    by (auto simp: twl_st_heur_state_simp twl_st_heur_isasat_fast_wl)
-  have H3:
-    \<open>RETURN (isasat_fast2 x) \<le> \<Down> {(b, b'). b = b' \<and> (b \<longrightarrow> isasat_fast2 x)} (SPEC (\<lambda>_. True))\<close>
-    for x
-     by (auto simp: RETURN_RES_refine_iff)
-  let ?R = \<open>{((b, brk, S), (b', brk', S')). b = b' \<and>
-       (b \<longrightarrow> isasat_fast2 S) \<and> brk = brk' \<and> (S, S') \<in> twl_st_heur}\<close>
-
-  show ?thesis
-    supply RETURN_as_SPEC_refine[refine2 del] twl_st_heur'_def[simp]
-    unfolding cdcl_twl_stgy_prog_break_wl_D_heur_break_def cdcl_twl_stgy_prog_break_wl_D_alt_def
-      isasat_fast2_def[symmetric]
-  apply (intro frefI nres_relI)
-  apply (refine_vcg H1 H2 H3
-      WHILEIT_refine[where R= ?R]
-      unit_propagation_outer_loop_wl_D_heur_unit_propagation_outer_loop_wl_D'[THEN fref_to_Down,
-        of x y \<open>dom_m (get_clauses_wl_heur x)\<close> for x y]
-      cdcl_twl_o_prog_wl_D_heur_cdcl_twl_o_prog_wl_D[THEN fref_to_Down]
-      cdcl_twl_stgy_prog_wl_D_heur_cdcl_twl_stgy_prog_wl_D[THEN fref_to_Down]
-      isasat_fast_slow_isasat_fast_slow_wl_D[THEN fref_to_Down, unfolded comp_def, simplified])
-  subgoal by (auto simp: twl_st_heur_state_simp twl_st_heur_isasat_fast_wl)
-  subgoal by (auto simp: twl_st_heur_state_simp twl_st_heur_isasat_fast_wl)
-  subgoal by (auto simp: twl_st_heur_state_simp)
-  subgoal by (auto simp: twl_st_heur_state_simp)
-  subgoal by (auto simp: twl_st_heur_state_simp)
-  subgoal by (auto simp: twl_st_heur_state_simp)
-  subgoal by (auto simp: twl_st_heur_state_simp isasat_fast2_def)
-  subgoal by (auto simp: twl_st_heur_state_simp)
-  subgoal by (auto simp: twl_st_heur_state_simp twl_st_heur_isasat_fast_wl)
-  subgoal by (auto simp: twl_st_heur_state_simp)
-  subgoal by (auto simp: twl_st_heur_state_simp twl_st_heur_isasat_fast_wl)
-  subgoal by (auto simp: twl_st_heur_state_simp twl_st_heur_isasat_fast_wl)
-  done
-
-qed *)
-
 end
 
-(* export_code cdcl_twl_stgy_prog_wl_D_fast_code in SML_imp module_name SAT_Solver
-  file "code/CDCL_Cached_Array_Trail_Fast.sml" *)
 
 export_code cdcl_twl_stgy_prog_wl_D_code in SML_imp module_name SAT_Solver
   file "code/CDCL_Cached_Array_Trail.sml"
